# CodeFigthsSolutions

int[] removeArrayPart(int[] inputArray, int l, int r) {
   if(inputArray.Length == 0) return inputArray;
return inputArray.Where((x,i)=>i<l||i>r).ToArray();
}


int[] replaceMiddle(int[] arr) {
int[] arr1 = new int[arr.Length-1];
        if(arr.Length%2 == 0)
               {
    for(int i =0; i< arr1.Length; i++)
    {
        if(i < arr.Length/2-1)
        {
                arr1[i] = arr[i];
        }
                    
        arr1[arr.Length/2-1] = arr[arr.Length/2 -1] + arr[arr.Length/2];
        
        if(i > arr.Length/2-1)
        {
                arr1[i] = arr[i+1]; 
        }
           
    }
  
 return arr1;
               }  else return arr;
}




int[] replaceMiddle(int[] arr) {
int n=arr.Length/2;
int[] arr1 = new int[n];
        int[] arr2 = new int[n-1];
        if(arr.Length%2 == 0)
               {
    for(int i =0; i< arr1.Length; i++)
    {
            arr1=arr.where((x,t)=>t<n-1).ToArray();
                            
        arr1[arr.Length/2-1] = arr[arr.Length/2 -1] + arr[arr.Length/2];
        
        arr2=arr.where((x,k)=>k>n/2).ToArray();
    }
  
 return arr1.Union(arr2).ToArray();
               }  else return arr;
}





///int[] replaceMiddle(int[] arr) {
int n=arr.Length;
        if(arr.Length%2 == 0)
              
               return (arr.where((x,t)=>t<n-1).ToArray()).Concat(new [] { arr.Skip(arr.Length/2-1).Take(2).Sum() }).Concat(arr.where((x,k)=>k>n/2).ToArray());
                            
         else return arr;
}


///int[] replaceMiddle(int[] arr) {
    return arr.Length % 2 == 1 ? arr :
        arr.Take(arr.Length/2-1)
            .Concat(new [] { arr.Skip(arr.Length/2-1).Take(2).Sum() })
            .Concat(arr.Skip(arr.Length/2+1))
            .ToArray();
}

